veric/semax_loop.v
@@ -224,10 +224,10 @@ Qed.
 Ltac inv_safe H :=
   inv H;
   try solve[match goal with
-    | H : j_at_external _ _ _ = _ |- _ =>
+    | H : semantics.at_external _ _ = _ |- _ =>
       simpl in H; congruence
-    | H : core_semantics.halted _ _ _ |- _ =>
-      contradiction
+    | H : semantics.halted _ _ = _ |- _ =>
+      simpl in H; unfold cl_halted in H; congruence
   end].
 (*
 Lemma seq_assoc2:
@@ -438,26 +438,24 @@ eapply guard_safe_adj; try apply H; try reflexivity. clear H.
 intros.
 destruct n; simpl in *. constructor.
 inv_safe H.
- {
   destruct (corestep_preservation_lemma Espec psi
           (Kseq Sskip :: k) k ora ve te m n (Kseq s) nil c' m')
-    as [c2 [m2 [? ?]]]; simpl; auto.
-  { intros. apply control_suffix_safe; simpl; auto.
-    clear.
-    intro; intros.
-    eapply convergent_controls_jsafe; try apply H0; simpl; auto.
-    intros.
-    destruct H1 as [H1 [H1a H1b]]; split3; auto.
-    inv H1; auto. }
-  { clear.
-     hnf; intros.
-     eapply convergent_controls_jsafe; try apply H0; simpl; auto.
-     clear; intros.
-     destruct H as [H1 [H1a H1b]]; split3; auto.
-     solve[inv H1; auto]. }
-   { destruct H1 as (?&?&?). econstructor; eauto. inv H. auto. }
-   { econstructor; eauto. }
-}
+  as [c2 [m2 [? ?]]]; simpl; auto.
+{ intros. apply control_suffix_safe; simpl; auto.
+clear.
+intro; intros.
+eapply convergent_controls_jsafe; try apply H0; simpl; auto.
+intros.
+destruct H1 as [H1 [H1a H1b]]; split3; auto.
+inv H1; auto. }
+{ clear.
+hnf; intros.
+eapply convergent_controls_jsafe; try apply H0; simpl; auto.
+clear; intros.
+destruct H as [H1 [H1a H1b]]; split3; auto.
+solve[inv H1; auto]. }
+{ destruct H1 as (?&?&?). econstructor; eauto. inv H. auto. }
+econstructor; eauto.
 Qed.
 
 Lemma semax_skip_seq {CS: compspecs}:
@@ -692,6 +690,91 @@ Proof.
       apply age1_ghost_of; auto.
   } Unfocus.
   apply assert_safe_jsafe; auto.
+Qed.
+
+Fixpoint nojumps s :=
+ match s with
+ | Ssequence s1 s2 => if nojumps s1 then nojumps s2 else false
+ | Sifthenelse _ s1 s2 => if nojumps s1 then nojumps s2 else false
+ | Sset _ _ => true
+ | Sassign _ _ => true
+ | Sskip => true
+ | _ => false
+end.
+
+Fixpoint nocontinue s :=
+ match s with
+ | Ssequence s1 s2 => if nocontinue s1 then nocontinue s2 else false
+ | Sifthenelse _ s1 s2 => if nocontinue s1 then nocontinue s2 else false
+ | Sswitch _ sl => nocontinue_ls sl
+ | Sgoto _ => false
+ | Scontinue => false
+ | _ => true
+end
+with nocontinue_ls sl :=
+ match sl with LSnil => true | LScons _ s sl' => if nocontinue s then nocontinue_ls sl' else false
+ end.
+
+Lemma jsafeN_relate_semax:
+ forall {CS: compspecs} s1 s2,
+ (forall OK_spec psi n (ora: OK_ty) vx b k jm,
+  jsafeN OK_spec psi n ora (State vx b (Kseq s2 :: k)) jm ->
+  jsafeN OK_spec psi n ora (State vx b (Kseq s1 :: k)) jm) ->
+forall  Delta P R,
+ (forall F, closed_wrt_modvars s1 F -> closed_wrt_modvars s2 F) ->
+ exit_tycon s1 = exit_tycon s2 ->
+ semax Espec Delta P s2 R ->
+ semax Espec Delta P s1 R.
+Proof.
+intros.
+rewrite semax_unfold in H2|-*.
+intros.
+specialize (H2 psi Delta' w TS HGG Prog_OK k F).
+specialize (H2 (H0 _ H3)).
+rewrite <- H1 in H2; specialize (H2 H4).
+clear - H2 H.
+hnf in H2|-*.
+intros b vx rho H5 H6 H7 H8.
+specialize (H2 b vx rho H5 H6 H7 H8).
+clear - H2 H.
+hnf in H2|-*.
+intros.
+specialize (H2 c H0).
+destruct H2 as [b0 [? ?]];
+exists b0; split; auto.
+destruct H2 as [m' [? [? [? ?]]]].
+exists m'; split3; auto.
+split; auto.
+simpl in H5|-*.
+intros.
+apply  H; auto.
+Qed.
+
+Lemma semax_loop_incr_into_body_equisafe:
+ forall body incr OK_spec psi n (ora: OK_ty) vx tx k jm,
+ nocontinue body = true ->
+ nojumps incr = true ->
+jsafeN OK_spec psi n ora
+      (State vx tx (Kseq (Sloop (Ssequence body incr) Sskip) :: k)) jm ->
+jsafeN OK_spec psi n ora (State vx tx (Kseq (Sloop body incr) :: k)) jm.
+Admitted.
+
+Lemma semax_loop_nocontinue:
+ forall {CS: compspecs} Delta P body incr R,
+ nocontinue body = true ->
+ nojumps incr = true ->
+ semax Espec Delta P (Ssequence body incr) (loop1_ret_assert P R) ->
+ semax Espec Delta P (Sloop body incr) R.
+Proof.
+  intros ? ? ? ? ?  POST Hbody Hincr H.
+  apply jsafeN_relate_semax with (Sloop (Ssequence body incr) Sskip); auto.
+2: apply semax_loop with P; auto;
+ eapply semax_post; try apply semax_skip;
+   intros; normalize; destruct POST; simpl; try apply derives_refl.
+ clear - Hbody Hincr.
+ intros.
+ rename b into tx.
+ apply semax_loop_incr_into_body_equisafe; auto.
 Qed.
 
 Lemma semax_break {CS: compspecs}:
